Partial verification of Partition.find
Things yet to do:

- Prove the height is correct (the first specification was wrong so a
  new one is needed)
- Finish verifying `Repair`

Partition.dfy
@@ -1,6 +1,8 @@
+include "Tree.dfy"
+
 class EquivClass {
-  ghost var repr: set<object>;
-  var height: nat;
+  ghost var repr: set<EquivClass>;
+  // var height: nat;
   var parent: EquivClass?;
 
   predicate Valid()
@@ -8,11 +10,11 @@ class EquivClass {
   {
     if parent == null then
       repr == {this}
-      && height == 0
+      // && height == 0
     else
       parent in repr
       && this !in parent.repr
-      && height == 1 + parent.height
+      // && height == 1 + parent.height  // MAL
       && repr == {this} + parent.repr
       // && repr >= {this} + parent.repr
       && parent.Valid()
@@ -23,90 +25,97 @@ class EquivClass {
     ensures parent == null
     ensures fresh(repr)
   {
-    height := 0;
+    // height := 0;
     parent := null;
     repr := {this};
   }
 
   predicate IsChildOf(p: EquivClass)
     reads this, repr
-    requires Valid()
+    // requires Valid()
+  {
+    parent == p
+  }
+
+  // The reflexive-transitive closure of `IsChildOf` (on valid EquivClasses)
+  predicate IsDescOf(p: EquivClass)
+    reads this, repr
+    // requires Valid()
   {
     p in repr
   }
 
-  static lemma IsChildOfRefl(a: EquivClass)
+  static lemma IsDescOfRefl(a: EquivClass)
     requires a.Valid()
-    ensures a.IsChildOf(a)
+    ensures a.IsDescOf(a)
   {}
 
-  static lemma IsChildOfWeakenRight(a: EquivClass, b: EquivClass)
-    requires a.Valid() && b.Valid()
-    requires b.parent != null
-    requires a.IsChildOf(b)
-    ensures a.IsChildOf(b.parent)
+  // static lemma IsDescOfWeakenRight(a: EquivClass, b: EquivClass)
+  //   requires a.Valid() && b.Valid()
+  //   requires b.parent != null
+  //   requires a.IsDescOf(b)
+  //   ensures a.IsDescOf(b.parent)
 
-  static lemma IsChildOfWeakenLeft(a: EquivClass, b: EquivClass)
-    requires a.Valid() && b.Valid()
-    requires a.parent != null
-    requires a.IsChildOf(b)
-    ensures a.parent.IsChildOf(b)
+  // static lemma IsDescOfWeakenLeft(a: EquivClass, b: EquivClass)
+  //   requires a.Valid() && b.Valid()
+  //   requires a.parent != null
+  //   requires a.IsDescOf(b)
+  //   ensures a.parent.IsDescOf(b)
 
-  static lemma IsChildOfWeakenLeftPrime(a: EquivClass, b: EquivClass)
-    requires a.Valid() && b.Valid()
-    requires a.parent != null
-    requires !a.parent.IsChildOf(b)
-    ensures !a.IsChildOf(b)
-  {
-    if a.IsChildOf(b) {
-      IsChildOfWeakenLeft(a, b);
-    }
-  }
-
-  static lemma IsChildOfTrans(a: EquivClass, b: EquivClass, c: EquivClass)
-    decreases a.repr
-    requires a.Valid() && b.Valid() && c.Valid()
-    requires a.IsChildOf(b) && b.IsChildOf(c)
-    ensures a.IsChildOf(c)
-  {
-    if a.parent != null && a != b {
-      IsChildOfTrans(a.parent, b, c);
-    }
-  }
-
-  static lemma IsChildOfAntisym(a: EquivClass, b: EquivClass)
-    decreases b.repr
-    requires a.Valid() && b.Valid()
-    requires a != b
-    requires a.IsChildOf(b)
-    ensures !b.IsChildOf(a)
-  {
-    if b.parent != a && b.parent != null {
-      IsChildOfWeakenRight(a, b);
-      IsChildOfAntisym(a, b.parent);
-    }
-  }
-
-  // static lemma IsChildOfTransPrime(a: EquivClass, b: EquivClass, c: EquivClass)
-  //   decreases a.repr
-  //   requires a.Valid() && b.Valid() && c.Valid()
-  //   requires !a.IsChildOf(b) && b.IsChildOf(c)
-  //   ensures !a.IsChildOf(c)
+  // static lemma IsDescOfWeakenLeftPrime(a: EquivClass, b: EquivClass)
+  //   requires a.Valid() && b.Valid()
+  //   requires a.parent != null
+  //   requires !a.parent.IsDescOf(b)
+  //   ensures !a.IsDescOf(b)
   // {
-  //   if a.parent != null && a != b {
-  //     if a != c {
-  //       IsChildOfTransPrime(a.parent, b, c);
-  //     } else {
-  //       assert !a.IsChildOf(b);
-  //       assert b.IsChildOf(a);
-  //       IsChildOfAntisym(b, a);
-  //       // assert a.IsChildOf(b);
-  //       assert !a.IsChildOf(a);
-  //       assert !a.IsChildOf(c);
-  //     }
+  //   if a.IsDescOf(b) {
+  //     IsDescOfWeakenLeft(a, b);
   //   }
   // }
 
+  static lemma IsDescOfTrans(a: EquivClass, b: EquivClass, c: EquivClass)
+    decreases a.repr
+    requires a.Valid() && b.Valid() && c.Valid()
+    requires a.IsDescOf(b) && b.IsDescOf(c)
+    ensures a.IsDescOf(c)
+  {
+    if a.parent != null && a != b {
+      IsDescOfTrans(a.parent, b, c);
+    }
+  }
+
+  // static lemma IsDescOfAntisym(a: EquivClass, b: EquivClass)
+  //   decreases b.repr
+  //   requires a.Valid() && b.Valid()
+  //   requires a != b
+  //   requires a.IsDescOf(b)
+  //   ensures !b.IsDescOf(a)
+  // {
+  //   if b.parent != a && b.parent != null {
+  //     IsDescOfWeakenRight(a, b);
+  //     IsDescOfAntisym(a, b.parent);
+  //   }
+  // }
+
+  // static lemma IsDescOfTransPrime(a: EquivClass, b: EquivClass, c: EquivClass)
+  //   decreases a.repr
+  //   requires a.Valid() && b.Valid() && c.Valid()
+  //   requires !a.IsDescOf(b) && b.IsDescOf(c)
+  //   ensures !a.IsDescOf(c)
+  // {
+  //   if a.parent != null && a != b {
+  //     if a != c {
+  //       IsDescOfTransPrime(a.parent, b, c);
+  //     } else {
+  //       assert !a.IsDescOf(b);
+  //       assert b.IsDescOf(a);
+  //       IsDescOfAntisym(b, a);
+  //       // assert a.IsDescOf(b);
+  //       assert !a.IsDescOf(a);
+  //       assert !a.IsDescOf(c);
+  //     }
+  //   }
+  // }
 }
 
 function method BigUnion<A>(S: set<set<A>>): set<A>
@@ -118,6 +127,45 @@ function method elems<A>(l: array<A>): set<A>
   reads l
 {
   set x | x in l[..]
+}
+
+// class Tree {
+//   var root: EquivClass;
+//   var children: set<Tree>;
+
+//   constructor Node(r: EquivClass, cs: set<Tree>)
+//   {
+//     root := r;
+//     children := cs;
+//   }
+
+//   function method Elems(): set<EquivClass>
+//     reads this
+//   {
+//     {root} + set y, c | c in children && y in c.Elems() :: y
+//   }
+
+//   predicate Valid()
+//     decreases this
+//     // reads elemsTree(t)
+//     // reads set c | c in children :: c.root
+//     // reads set c | c in children :: c.root.parent
+//   {
+//     forall c | c in children ::
+//       c.root.parent == root
+//       // && c.root.height == p.height + 1
+//       && c.Valid()
+//   }
+// }
+
+predicate ValidTree(t: Tree<EquivClass>)
+  decreases t
+  reads set c | c in elemsTree(t) :: c`parent
+{
+  forall c | c in t.children ::
+    assert elemsTree(c) <= elemsTree(t);
+    c.root.parent == t.root
+    && ValidTree(c)
 }
 
 class Partition {
@@ -133,128 +181,274 @@ class Partition {
     reads this, classes, elems(classes), ValidReads()
   {
     (forall e: EquivClass | e in classes[..] ::
-      e.Valid() && (forall p: EquivClass | p in e.repr :: p in classes[..])
+      e.Valid()
     )
+    && (forall e: EquivClass, p: EquivClass | e in classes[..] && p in e.repr ::
+        p in classes[..]
+      )
     && (forall j, k | 0 <= j < k < classes.Length :: classes[j] != classes[k])
   }
 
-  constructor(size: nat)
-    ensures Valid()
-  {
-    new;  // ¿¿¿¿qué hace esto???? .-.
-    var i := 0;
-    var temp := new EquivClass?[size](_ => null);
-    while i < size
-      modifies temp
-      invariant 0 <= i <= size
-      invariant forall j | 0 <= j < i :: temp[j] != null
-      invariant forall j, k | 0 <= j < k < i :: temp[j] != temp[k]
-      invariant forall j | 0 <= j < i :: temp[j].parent == null && temp[j].Valid()
-    {
-      temp[i] := new EquivClass();
-      i := i + 1;
-    }
-    classes := new EquivClass[size](
-      i requires 0 <= i < size reads temp => temp[i]
-    );
-  }
-
-  lemma IsChildOfTransPrimeForall(a: EquivClass, c: EquivClass)
-    requires a.Valid() && c.Valid()
-    requires !a.IsChildOf(c)
-    ensures forall b | b in classes[..] :: a.IsChildOf(b) ==> !a.IsChildOf(c)
-
-  lemma IsChildOfTransPrimeForall2(a: EquivClass)
-    requires a.Valid()
-    requires Valid()
-    ensures forall b | b in classes[..] :: a.IsChildOf(b) ==> !b.IsChildOf(a)
-
-  function method ChildrenAuxAux(c: EquivClass, p: EquivClass):
-      (set<EquivClass>, bool)
-    decreases c.repr
-    reads this, classes, elems(classes), ValidReads()
-    requires Valid()
-    requires p in classes[..]
-    requires c in classes[..]
-    ensures forall e: EquivClass | e in classes[..]
-      :: e in ChildrenAuxAux(c, p).0 <==> c.IsChildOf(e) && e.IsChildOf(p)
-    ensures ChildrenAuxAux(c, p).1 <==> c.IsChildOf(p)
-  {
-    if c == p then
-      IsChildOfTransPrimeForall2(c);
-      ({c}, true)
-    else if c.parent == null then
-      ({}, false)
-    else
-      var rec := ChildrenAuxAux(c.parent, p);
-      if rec.1 then
-        (rec.0 + {c}, true)
-      else
-        EquivClass.IsChildOfWeakenLeftPrime(c, p);
-        IsChildOfTransPrimeForall(c, p);
-        rec
-  }
-
-  // function method ChildrenAux(i: nat, p: EquivClass): set<EquivClass>
-  //   reads this, classes, elems(classes), ValidReads()
-  //   decreases classes.Length - i
-  //   requires Valid()
-  //   requires i <= classes.Length
-  //   requires p in classes[..]
-  //   ensures forall e, d
-  //     | e in classes[i..] && d in classes[i..] && e.IsChildOf(d)
-  //     :: e in ChildrenAux(i, p) <==> e.IsChildOf(p)
+  // constructor(size: nat)
+  //   ensures Valid()
   // {
-  //   if i == classes.Length then
-  //     assert forall e: EquivClass
-  //       | e in classes[i..]
-  //       :: e in {} <==> e.IsChildOf(p);
-  //     {}
-  //   else
-  //     var c := classes[i];
-  //     var rec := ChildrenAux(i+1, p);
-  //     // if classes[i] in rec then
-  //     //   assert forall e: EquivClass
-  //     //     | e in classes[i..]
-  //     //     :: e in rec <==> e.IsChildOf(p);
-  //     //   rec
-  //     // else
-  //       assert forall e, d: EquivClass
-  //         | e in classes[i+1..] && d in classes[i+1..] && e.IsChildOf(d)
-  //         :: e in rec <==> e.IsChildOf(p);
-  //       assert forall e: EquivClass | e in classes[..]
-  //         :: e in ChildrenAuxAux(c, p).0 <==> c.IsChildOf(e) && e.IsChildOf(p);
-  //       assert forall e, d
-  //         | e in classes[i..] && d in classes[i..] && e.IsChildOf(d)
-  //         :: e in rec + ChildrenAuxAux(c, p).0 <==> e.IsChildOf(p);
-  //       // assert forall e: EquivClass
-  //       //   | e in classes[i..]
-  //       //   :: e in rec + ChildrenAuxAux(classes[i], p).0 <==> e.IsChildOf(p);
-  //       rec + ChildrenAuxAux(c, p).0
+  //   new;  // ¿¿¿¿qué hace esto???? .-.
+  //   var i := 0;
+  //   var temp := new EquivClass?[size](_ => null);
+  //   while i < size
+  //     modifies temp
+  //     invariant 0 <= i <= size
+  //     invariant forall j | 0 <= j < i :: temp[j] != null
+  //     invariant forall j, k | 0 <= j < k < i :: temp[j] != temp[k]
+  //     invariant forall j | 0 <= j < i :: temp[j].parent == null && temp[j].Valid()
+  //   {
+  //     temp[i] := new EquivClass();
+  //     i := i + 1;
+  //   }
+  //   classes := new EquivClass[size](
+  //     i requires 0 <= i < size reads temp => temp[i]
+  //   );
   // }
 
-  // function method ChildrenAux(i: nat, p: EquivClass): set<EquivClass>
-  //   reads this, classes, elems(classes), ValidReads()
-  //   decreases classes.Length - i
+  // lemma ReprSubSet(e: EquivClass)
+  //   requires e in classes[..]
   //   requires Valid()
-  //   requires i <= classes.Length
-  //   requires p in classes[..]
-  //   ensures forall e: EquivClass
-  //   | e in classes[i..]
-  //   :: e in ChildrenAux(i, p) <==> e.IsChildOf(p)
+  //   ensures multiset(e.repr) <= multiset(classes[..])
+
+  function Descendants(p: EquivClass): set<EquivClass>
+    reads this, classes, elems(classes), ValidReads()
+    // requires Valid()
+    requires p in classes[..]
+    // ensures Descendants(p)
+    //   == (set c: EquivClass | c in classes[..] && c.IsChildOf(p) :: c)
+  {
+    set c | c in classes[..] && c.IsDescOf(p)
+  }
 
   function Children(p: EquivClass): set<EquivClass>
     reads this, classes, elems(classes), ValidReads()
-    requires Valid()
+    // requires Valid()
     requires p in classes[..]
   {
-    set c | c in classes[..] && c.IsChildOf(p) :: c
+    set c | c in classes[..] && c.IsChildOf(p)
   }
+
+  lemma ChildDesc(c: EquivClass, p: EquivClass)
+    decreases c.repr
+    requires c in classes[..]
+    requires p in classes[..]
+    requires Valid()
+    ensures c.IsDescOf(p)
+      <==> c == p || exists d: EquivClass | d in classes[..] :: c.IsDescOf(d) && d.IsChildOf(p)
+  {
+    assert c.Valid();
+    assert p.Valid();
+    if c.IsDescOf(p) {
+      assert p in c.repr;
+      if c.parent == null {
+        assert c == p;
+      } else {
+        ChildDesc(c.parent, p);
+      }
+    }
+    if c == p {
+    }
+    if exists d | d in classes[..] :: c.IsDescOf(d) && d.IsChildOf(p) {
+      var d: EquivClass; d :| d in classes[..] && c.IsDescOf(d) && d.IsChildOf(p);
+      assert d.IsDescOf(p);
+      EquivClass.IsDescOfTrans(c, d, p);
+    }
+  }
+
+  lemma ChildrenDescendants(p: EquivClass)
+    requires p in classes[..]
+    requires Valid()
+    ensures Descendants(p)
+      == {p} + BigUnion(set c
+        | c in classes[..] && c.IsChildOf(p)
+        :: Descendants(c))
+  {
+    calc == {
+      Descendants(p);
+      set c | c in classes[..] && c.IsDescOf(p);
+      { forall c | c in classes[..]
+          ensures c.IsDescOf(p)
+            <==> c == p
+            || exists d: EquivClass | d in classes[..] :: c.IsDescOf(d) && d.IsChildOf(p)
+        {
+          ChildDesc(c, p);
+        }
+      }
+      set c
+        | c in classes[..]
+        && ( c == p
+          || exists d: EquivClass | d in classes[..] :: c.IsDescOf(d) && d.IsChildOf(p)
+          );
+      (set c | c in classes[..] && c == p)
+      + (set c
+          | c in classes[..]
+          && exists d: EquivClass | d in classes[..] :: c.IsDescOf(d) && d.IsChildOf(p)
+          );
+      {
+        assert (set c | c in classes[..] && c == p) == {p};
+      }
+      ({p} + set c
+        | c in classes[..]
+        && exists d: EquivClass | d in classes[..] :: c.IsDescOf(d) && d.IsChildOf(p));
+      ({p} + set c, d: EquivClass
+        | c in classes[..] && d in classes[..]
+        && d.IsDescOf(c) && c.IsChildOf(p)
+        :: d);
+      {
+        assert forall c, d: EquivClass
+          | c in classes[..]
+          :: d in Descendants(c)
+          <==> d in classes[..] && d.IsDescOf(c);
+      }
+      ({p} + set c, d | c in classes[..] && c.IsChildOf(p) && d in Descendants(c) :: d);
+      ({p} + BigUnion(set c
+        | c in classes[..] && c.IsChildOf(p)
+        :: Descendants(c)));
+    }
+  }
+
+  function DescendantsTree(p: EquivClass): Tree<EquivClass>
+    decreases elems(classes) - p.repr
+    reads this, classes, elems(classes), ValidReads()
+    requires Valid()
+    requires p in classes[..]
+    ensures elemsTree(DescendantsTree(p)) == Descendants(p)
+    ensures ValidTree(DescendantsTree(p))
+    // ensures forall c, d
+    //   | c in elemsTree(DescendantsTree(p))
+    //   && d in elemsTree(DescendantsTree(p))
+    //   && c.IsDescOf(d)
+    //   :: c !in d.repr
+  {
+    ChildrenDescendants(p);
+    Node(
+      p,
+      set c: EquivClass | c in classes[..] && c.IsChildOf(p) ::
+        DescendantsTree(c)
+    )
+  }
+
+  // ghost method RepairDescendants(p: EquivClass, dt: Tree<EquivClass>)
+  //   modifies p, elemsTree(dt)
+  //   requires p in classes[..]
+  //   requires p.Valid()
+  //   requires elemsTree(dt) == Descendants(p)
+  //   ensures forall c | c in elemsTree(dt) :: c.Valid()
+  // {
+  //   match dt {
+  //     case Node(p_, cs) => {
+  //       // assert p_ == p;
+  //       var children := {};
+  //       while cs - children != {}
+  //         decreases cs - children
+  //         modifies BigUnion(set c | c in cs :: elemsTree(c))
+  //         invariant forall c | c in children ::
+  //           c.root.Valid() && forall d | d in elemsTree(dt) :: d.Valid()
+  //       {
+  //         var c;
+  //         c :| c in (cs - children);
+  //         c.root.repr := {c.root} + p.repr;
+  //         RepairDescendants(c.root, c);
+  //         children := children + {c};
+  //       }
+  //     }
+  //   }
+  // }
+
+  // ghost method RepairChild(p: EquivClass, dt: Tree<EquivClass>)
+  //   modifies elemsTree(dt)
+  //   requires dt.root.IsChildOf(p)
+  //   ensures ValidTree(dt)
+
+  ghost method RepairDescendants(dt: Tree<EquivClass>)
+    modifies dt.root, elemsTree(dt)
+    requires forall c | c in elemsTree(dt) :: c in classes[..]
+    requires dt.root.Valid()
+    requires ValidTree(dt)
+    // requires forall c | c != dt.root && c in elemsTree(dt) :: c !in dt.root.repr
+    // requires forall c, d | c in elemsTree(dt) && d in elemsTree(dt) && c.IsDescOf(d) ::
+    //   c !in d.repr
+    requires forall c, d | c in elemsTree(dt) && d in elemsTree(dt) && c.IsChildOf(d) ::
+      c !in d.repr
+    ensures forall c, d | c in elemsTree(dt) && d in elemsTree(dt) && c.IsChildOf(d) ::
+      c !in d.repr
+    ensures forall c | c in elemsTree(dt) :: c.Valid()
+    ensures ValidTree(dt)
+  {
+    match dt {
+      case Node(p, cs) => {
+        var children := {};
+        while cs - children != {}
+          decreases cs - children
+          // modifies set c, d | c in cs && d in elemsTree(c) :: d`repr
+          invariant children <= cs
+          invariant Node(p, cs) == dt
+          invariant p.Valid()
+          invariant ValidTree(dt)
+          invariant forall c, d
+            | c in elemsTree(dt) && d in elemsTree(dt) && c.IsChildOf(d)
+            :: c !in d.repr
+          invariant forall c, d | c in children && d in elemsTree(c) :: d.Valid()
+        {
+          assert forall c, d
+            | c in elemsTree(dt) && d in elemsTree(dt) && c.IsChildOf(d)
+            :: c !in d.repr;
+          var ct; ct :| ct in cs - children;
+          // assert forall a | a in cs :: elemsTree(a) <= elemsTree(dt);
+          assert ct.root in elemsTree(ct);
+          assert ct.root.IsChildOf(p);
+          assert ct.root !in p.repr;
+          ct.root.repr := {ct.root} + p.repr;
+          // assert (set c | c in elemsTree(dt) :: c.repr)
+          //   <= (set a, b | a in cs && b in elemsTree(a) :: b.repr);
+          // assert forall d | d in elemsTree(c) :: d in elemsTree(dt);
+          assert elemsTree(ct) <= elemsTree(dt);
+          assert ct.root.parent == p;
+          assert p.Valid();
+          assert ct.root.parent.Valid();
+          assert ct.root.Valid();
+          assert forall c, d
+            | c in elemsTree(dt) && d in elemsTree(dt) && c.IsChildOf(d)
+            :: c !in d.repr;
+          assert forall c, d
+            | c in elemsTree(ct) && d in elemsTree(ct) && c.IsChildOf(d)
+            :: c !in d.repr;
+          RepairDescendants(ct);
+          assert forall c, d
+            | c in elemsTree(ct) && d in elemsTree(ct) && c.IsChildOf(d)
+            :: c !in d.repr;
+          assert forall c, d
+            | c in elemsTree(dt) && d in elemsTree(dt) && c.IsChildOf(d)
+            :: c !in d.repr;
+          assert ct.root.Valid();
+          assert forall d | d in elemsTree(ct) :: d.Valid();
+          children := children + {ct};
+        }
+        assert cs - children == {};
+        assert children <= cs;
+        assert cs - children + children == {} + children;
+        assert cs == children;
+      }
+    }
+  }
+
+  // ghost method repair(e: EquivClass, c: EquivClass, top: EquivClass)
+  //   modifies e
+  // {
+  //   e.repr := e.repr - c.repr;
+  //   e.repr := e.repr + {c, top};
+  // }
 
   /*
   method findAux(c: EquivClass) returns (res: EquivClass)
     decreases c.repr
-    modifies c, c.repr
+    modifies multiset(classes[..])
+    requires c in classes[..]
     requires Valid()
     requires c.Valid()
     ensures res in old(c.repr)
@@ -263,20 +457,50 @@ class Partition {
     ensures c.Valid()
     ensures c.parent == null || c.parent == res
     ensures Valid()
+    ensures forall e | e in old(classes[..]) :: e in classes[..]
   {
     if c.parent == null {
       return c;
     } else {
       res := findAux(c.parent);
+      assert res.Valid();
       assert Valid();
+      ghost var dt := DescendantsTree(c);
       c.parent := res;
-      c.height := 1;
+      // c.height := 1;
+      ghost var orepr := c.repr;
       c.repr := {c, res};
       assert c.Valid();
+      ghost var cs: set<EquivClass> := Descendants(c);
+      assert forall e | e in cs :: e in multiset(classes[..]);
+      // while cs != {}
+      //   decreases cs
+      //   invariant res.Valid()
+      //   invariant c.Valid()
+      //   invariant forall e | e in old(classes[..]) :: e in classes[..]
+      //   invariant forall e | e in classes[..] && e !in cs :: e.Valid()
+      //   invariant forall e: EquivClass, p: EquivClass | e in classes[..] && p in e.repr ::
+      //     p in classes[..]
+      //   invariant forall j, k | 0 <= j < k < classes.Length :: classes[j] != classes[k]
+      // {
+      //   var e: EquivClass;
+      //   e :| e in cs;
+      //   if c in e.repr {
+      //     e.repr := e.repr - c.repr;
+      //     e.repr := e.repr + {c, res};
+      //   }
+      //   cs := cs - {e};
+      // }
+      assert forall e | e in classes[..] && e !in cs :: e.Valid();
+      RepairDescendants(dt);
+      assert forall e | e in cs :: e.Valid();
+      assert forall e: EquivClass | e in classes[..] :: e.Valid();
       assert Valid();
     }
   }
+     */
 
+  /*
   method find(i: nat) returns (res: EquivClass)
     modifies this, elems
     modifies set x | x in elems[..]
