Tree.dfy
@@ -1,0 +1,38 @@
+datatype Tree<A(==)>
+  = Node(root: A, children: set<Tree<A>>)
+
+function method elemsTree<A>(t: Tree<A>): set<A>
+{
+  match t {
+    // case Empty => {}
+    case Node(x, children) => {x} + set y, c | c in children && y in elemsTree(c) :: y
+  }
+}
+
+// function method MapMultiSet<A, B>(f: A -> B, m: multiset<A>): multiset<B>
+// {
+//   if e :| e in m then
+//     multiset{f(e)} + MapMultiSet(f, m - multiset{e})
+//   else
+//     multiset{}
+// }
+
+// function method UnionMultiSet<A>(m: multiset<multiset<A>>): multiset<A>
+// {
+//   if s :| s in m then
+//     s + UnionMultiSet(m - multiset{s})
+//   else
+//     multiset{}
+// }
+
+// function method melems<A>(t: Tree<A>): multiset<A>
+// {
+//   match t {
+//     case Empty => {}
+//     case Node(x, children) =>
+//       multiset{x}
+//       + if children == multiset{} then
+//           {}
+//         else
+//   }
+// }
